higher gref

pulse/src/checker/Pulse.Lib.Core.Typing.fsti
@@ -478,3 +478,14 @@ val gref_non_informative_witness_typing
   (t_typing:RT.tot_typing g t (pack_ln (Tv_Type uzero)))
   : GTot (RT.tot_typing g (gref_non_informative_witness_tm t)
                           (non_informative_witness_rt uzero (mk_gref uzero t)))
+
+let higher_gref_non_informative_witness_tm (t:term) : term =
+  let tm = pack_ln (Tv_UInst (pack_fv higher_gref_non_informative_lid) [uone]) in
+  pack_ln (Tv_App tm (t, Q_Explicit))
+
+val higher_gref_non_informative_witness_typing
+  (#g:env)
+  (#t:term)
+  (t_typing:RT.tot_typing g t (pack_ln (Tv_Type uone)))
+  : GTot (RT.tot_typing g (higher_gref_non_informative_witness_tm t)
+                          (non_informative_witness_rt uzero (mk_higher_gref uone t)))
